floyd/canon.v
@@ -2136,6 +2136,9 @@ Inductive return_outer_gen: ret_assert -> ret_assert -> Prop :=
 | return_outer_gen_loop1: forall inv P Q,
     return_outer_gen P Q ->
     return_outer_gen (loop1_ret_assert inv P) Q
+| return_outer_gen_loop1a: forall inv P Q,
+    return_outer_gen P Q ->
+    return_outer_gen (loop1a_ret_assert inv P) Q
 | return_outer_gen_loop2: forall inv P Q,
     return_outer_gen P Q ->
     return_outer_gen (loop2_ret_assert inv P) Q.
