progs/verif_strlib.v
@@ -78,34 +78,6 @@ Definition Gprog : funspecs :=
 (* Often an if statement only serves to add information (e.g., rule out some cases). *)
 Ltac forward_if_prop P := match goal with |-semax _ (PROP () ?Q) _ _ => forward_if (PROP (P) Q) end.
 
-Lemma zero_in_body: forall i ls, ~In 0 ls -> Znth i (ls ++ [0]) 0 = 0 -> 0 <= i < Zlength ls -> forall P, P.
-Proof.
-intros.
-contradiction H.
-rewrite app_Znth1 in H0 by omega. rewrite <- H0. apply Znth_In. auto.
-Qed.
-
-
-Lemma Znth_zero_zero:
-  forall i {A} (a: A), Znth i [a] a = a.
-Proof.
-intros.
-unfold Znth.
-if_tac; auto. destruct (Z.to_nat i). reflexivity. destruct n; reflexivity.
-Qed.
-
-Ltac zero_in_body := 
-  pose_Zlength_nonneg;
-  apply Classical_Prop.NNPP; intro;
-  match goal with
-  | H: ~In 0 ?ls, H1: Znth ?i (?ls' ++ [0]) 0 = 0 |- _ =>
-     constr_eq ls ls'; elimtype False; apply H; rewrite <- H1; 
-    rewrite app_Znth1 by omega; apply Znth_In; omega
-  | H: ~In 0 ?ls, H1: Znth ?i (?ls' ++ [0]) 0 <> 0 |- _ =>
-     constr_eq ls ls'; elimtype False; apply H1;
-    rewrite app_Znth2 by omega; apply Znth_zero_zero
- end.
-
 Hint Rewrite Z.add_simpl_r Z.sub_simpl_r : norm entailer_rewrite.
 
 Lemma body_strlen: semax_body Vprog Gprog f_strlen strlen_spec.
@@ -135,98 +107,15 @@ assert (Zlength (ls ++ [0]) = Zlength ls + 1) by (autorewrite with sublist; auto
 forward.
 forward_if.
 forward.
-entailer!. f_equal. f_equal. zero_in_body.
+entailer!. f_equal. f_equal. cstring.
 forward.
 Exists (i+1).
-entailer!. zero_in_body.
+entailer!. cstring.
 *
 Intros i.
 forward.
 Exists i.
 entailer!.
-Qed.
-
-Lemma insert_PROP:
- forall (P: Prop) (L: list Prop) Q, P -> PROPx L Q = PROPx (P::L) Q.
-Proof.
-intros.
-unfold PROPx.
-f_equal. f_equal. simpl. apply prop_ext. intuition.
-Qed.
-
-Ltac revert_PROP :=
- match goal with 
- | H: ?P |- ENTAIL _, PROPx ?L ?Q |-- _ =>
-    match type of P with Prop => 
-      rewrite (insert_PROP P L Q) by apply H; clear H
-    end
- end.
-
-
-Lemma body_strchr': semax_body Vprog Gprog f_strchr strchr_spec.
-  (* Alternate proof of strchar to demonstrate handling
-    of "continue:" using an evar.  Not very easy... *)
-Proof.
-start_function.
-forward.
-unfold cstring.
-set (ls := string_to_Z s) in *.
-Intros.
-evar (Q: Z -> environ->mpred).
-forward_loop (EX i : Z,
-  PROP (0 <= i < Zlength ls + 1; Forall (fun d => d <> c) (sublist 0 i ls))
-  LOCAL (temp _str str; temp _c (Vint (Int.repr c)); temp _i (Vint (Int.repr i)))
-  SEP (data_at Tsh (tarray tschar (Zlength ls + 1))
-          (map Vint (map Int.repr (ls ++ [0]))) str))
- continue: (EX i:Z, Q i).
-  Exists 0; rewrite sublist_nil; entailer!.
-- Intros i. 
-  pose proof (repable_string_i s i) as Hi; fold ls in Hi.
-  forward.
-  assert (Zlength (ls ++ [0]) = Zlength ls + 1) by (autorewrite with sublist; auto).
-  forward.
-  forward.
-  forward_if_prop (Znth i (ls ++ [0]) 0 <> c).
-  { rewrite data_at_isptr; Intros.
-    forward. 
-    Exists (offset_val i str).
-    unfold cstring. fold ls. 
-    entailer!.
-    left. exists i. split3; auto.
-    destruct (zlt i (Zlength ls)); autorewrite with sublist in *; simpl in *; auto.
-    assert (i = Zlength ls) by omega. subst i.
-    rewrite Z.sub_diag in *. contradiction H0. reflexivity. }
-  { forward.
-    entailer!. }
-  Intros.
-  forward_if_prop (Znth i (ls ++ [0]) 0 <> 0).
-  { rewrite data_at_isptr; Intros.
-    forward.
-    Exists (Vint Int.zero); unfold cstring; rewrite !map_app; entailer!.
-    right. split; auto.
-    assert (i = Zlength ls). {
-      destruct (zlt i (Zlength ls)); [ | omega].
-      contradiction H1. rewrite app_Znth1 in H6 by omega.
-      rewrite <- H6. apply Znth_In. omega.
-    }
-    subst i.
-    autorewrite with sublist in H3; auto. }
-  { forward.
-    entailer!. }
-  subst Q. Exists i. repeat revert_PROP. apply ENTAIL_refl.
--
-  subst Q. cbv beta.
-  Intros i.
-  deadvars!.
-  forward.
-  Exists (i+1).
-  entailer!.
-  assert (i <> Zlength ls)
-     by(intro; subst i; apply H7; autorewrite with sublist; reflexivity).
-  split. rep_omega.
-  rewrite (sublist_split 0 i) by rep_omega. rewrite Forall_app. split; auto.
-  rewrite sublist_len_1 with (d:=0) by rep_omega. repeat constructor.
-  rewrite app_Znth1 in H6 by rep_omega. auto.
 Qed.
 
 Lemma body_strchr: semax_body Vprog Gprog f_strchr strchr_spec.
@@ -257,7 +146,7 @@ forward_loop (EX i : Z,
   { forward. 
     Exists (offset_val i str).
     entailer!.
-    left. exists i. split3; auto. rewrite app_Znth1; auto. zero_in_body. }
+    left. exists i. split3; auto. rewrite app_Znth1; auto. cstring. }
   { forward.
     entailer!. }
   Intros.
@@ -265,12 +154,12 @@ forward_loop (EX i : Z,
   { forward.
     Exists nullval; rewrite !map_app; entailer!.
     right. split; auto.
-    assert (i = Zlength ls) by zero_in_body.
+    assert (i = Zlength ls) by cstring.
     subst i.
     autorewrite with sublist in H3; auto. }
   forward.
   Exists (i+1); entailer!.
-  assert (i <> Zlength ls) by zero_in_body.
+  assert (i <> Zlength ls) by cstring.
   split. omega.
   rewrite (sublist_split 0 i) by rep_omega. rewrite Forall_app. split; auto.
   rewrite sublist_len_1 with (d:=0) by rep_omega. repeat constructor.
@@ -371,10 +260,10 @@ forward_loop (EX i : Z,
   forward.
   forward_if.
   + forward.
-    entailer!. f_equal. f_equal. zero_in_body.
+    entailer!. f_equal. f_equal. cstring.
   +
     forward.
-    Exists (i+1); entailer!. zero_in_body.
+    Exists (i+1); entailer!. cstring.
 - Intros i.
    forward.
    Exists i. entailer!. 
@@ -424,7 +313,7 @@ forward_loop (EX i : Z,
       rewrite prop_true_andp 
         by (intro Hx; apply in_app in Hx; destruct Hx; contradiction).
       cancel.
-    assert (j = Zlength ls) by zero_in_body; subst.
+    assert (j = Zlength ls) by cstring; subst.
     autorewrite with sublist.
     apply derives_refl'.
     unfold data_at; f_equal. 
@@ -439,7 +328,7 @@ forward_loop (EX i : Z,
  +
   forward.
   Exists (j+1).
-  destruct (zlt j (Zlength ls)); [ | zero_in_body].
+  destruct (zlt j (Zlength ls)); [ | cstring].
   entailer!.
   change (field_at Tsh (tarray tschar n) []) with (data_at Tsh (tarray tschar n)).
   rewrite (sublist_split 0 j (j+1)) by rep_omega.
@@ -495,11 +384,11 @@ forward_loop (EX i : Z,
   assert (Znth i (ls1 ++ [0]) 0 = 0 <-> i = Zlength ls1) as Hs1.
   { split; [|intro; subst; rewrite app_Znth2, Zminus_diag by omega; auto].
     destruct (zlt i (Zlength ls1)); [|omega].
-    intro X; lapply (Znth_In i ls1 0); [|omega]. zero_in_body. }
+    intro X; lapply (Znth_In i ls1 0); [|omega]. cstring. }
   assert (Znth i (ls2 ++ [0]) 0 = 0 <-> i = Zlength ls2) as Hs2.
   { split; [|intro; subst; rewrite app_Znth2, Zminus_diag by omega; auto].
     destruct (zlt i (Zlength ls2)); [|omega].
-    intro X; lapply (Znth_In i ls2 0); [|omega]. zero_in_body. }
+    intro X; lapply (Znth_In i ls2 0); [|omega]. cstring. }
   forward.
   forward.
   match goal with |-semax _ (PROP () (LOCALx ?Q ?R)) _ _ =>
@@ -510,7 +399,7 @@ forward_loop (EX i : Z,
     rewrite Hs1 in *.
     destruct (zeq (Znth i (ls2 ++ [0]) 0) 0).
     + rewrite e; simpl force_val.
-         assert (i = Zlength ls2) by zero_in_body.
+         assert (i = Zlength ls2) by cstring.
         rewrite  (proj2 Hs1 H6).
      rewrite (proj2 (Z.eqb_eq i (Zlength ls1)) H6).
      rewrite (proj2 (Z.eqb_eq i (Zlength ls2)) H7).
@@ -633,7 +522,7 @@ forward_loop (EX i : Z,
  forward_if.
 + forward.
    entailer!.
-  assert (i = Zlength ls) by zero_in_body. subst i.
+  assert (i = Zlength ls) by cstring. subst i.
   change (field_at Tsh (tarray tschar n) []) with (data_at Tsh (tarray tschar n)).
   rewrite upd_Znth_app2 by list_solve.
   autorewrite with sublist.
@@ -648,7 +537,7 @@ forward_loop (EX i : Z,
   rewrite !split_data_at_app_tschar by list_solve.
   cancel.
 +
-   assert (i < Zlength ls) by zero_in_body.
+   assert (i < Zlength ls) by cstring.
   forward.
   Exists (i+1). entailer!. 
   autorewrite with sublist.
@@ -673,4 +562,422 @@ forward_loop (EX i : Z,
   Exists i.
   entailer!.
 Qed.
+
+Module Alternate.
+
+(* Alternate proofs of these functions, using the form of "forward_loop"
+  that relies on semax_loop_nocontinue *)
+
+
+Lemma body_strlen: semax_body Vprog Gprog f_strlen strlen_spec.
+Proof.
+start_function.
+unfold cstring in *.
+set (ls := string_to_Z s) in *.
+Intros.
+forward.
+forward_loop (EX i : Z,
+  PROP (0 <= i < Zlength ls + 1)
+  LOCAL (temp _str str; temp _i (Vptrofs (Ptrofs.repr i)))
+  SEP (data_at Tsh (tarray tschar (Zlength ls + 1))
+          (map Vint (map Int.repr (ls ++ [0]))) str)).
+*
+Exists 0. entailer!.
+*
+
+Intros i.
+forward.
+assert (Hi := repable_string_i s i); fold ls in Hi.
+assert (Zlength (ls ++ [0]) = Zlength ls + 1) by (autorewrite with sublist; auto).
+forward.
+
+forward_if_prop (Znth i (ls ++ [0]) 0 <> 0).
+forward.
+entailer!. f_equal. f_equal. cstring.
+forward.
+entailer!.
+forward.
+Exists (i+1).
+entailer!. cstring.
+Qed.
+
+Lemma body_strchr: semax_body Vprog Gprog f_strchr strchr_spec.
+Proof.
+start_function.
+forward.
+unfold cstring in *.
+set (ls := string_to_Z s) in *.
+Intros.
+forward_loop (EX i : Z,
+  PROP (0 <= i < Zlength ls + 1; Forall (fun d => d <> c) (sublist 0 i ls))
+  LOCAL (temp _str str; temp _c (Vint (Int.repr c)); temp _i (Vint (Int.repr i)))
+  SEP (data_at Tsh (tarray tschar (Zlength ls + 1))
+          (map Vint (map Int.repr (ls ++ [0]))) str)).
+  Exists 0; rewrite sublist_nil; entailer!.
+- Intros i. 
+  pose proof (repable_string_i s i) as Hi; fold ls in Hi.
+  forward.
+  assert (Zlength (ls ++ [0]) = Zlength ls + 1) by (autorewrite with sublist; auto).
+  forward.
+  forward.
+  forward_if_prop (Znth i (ls ++ [0]) 0 <> c).
+  { forward. 
+    Exists (offset_val i str).
+    entailer!.
+    left. exists i. split3; auto. rewrite app_Znth1; auto. cstring. }
+  { forward.
+    entailer!. }
+  Intros.
+  forward_if_prop (Znth i (ls ++ [0]) 0 <> 0).
+  { forward.
+    Exists nullval; rewrite !map_app; entailer!.
+    right. split; auto.
+    assert (i = Zlength ls) by cstring.
+    subst i.
+    autorewrite with sublist in H3; auto. }
+  forward.
+  entailer!.
+  forward.
+  Exists (i+1); entailer!.
+  assert (i <> Zlength ls) by cstring.
+  split. omega.
+  rewrite (sublist_split 0 i) by rep_omega. rewrite Forall_app. split; auto.
+  rewrite sublist_len_1 with (d:=0) by rep_omega. repeat constructor.
+  rewrite app_Znth1 in H5 by rep_omega. auto.
+Qed.
+
+Lemma split_data_at_app:
+ forall sh t n (al bl: list (reptype t)) abl'
+         (al': reptype (tarray t (Zlength al)))
+         (bl': reptype (tarray t (n - Zlength al)))
+          p ,
+   n = Zlength (al++bl) ->
+   JMeq abl' (al++bl) ->
+   JMeq al' al ->
+   JMeq bl' bl ->
+   data_at sh (tarray t n) abl' p = 
+         data_at sh (tarray t (Zlength al)) al' p
+        * data_at sh (tarray t (n - Zlength al)) bl'
+                 (field_address0 (tarray t n) [ArraySubsc (Zlength al)] p).
+Proof.
+intros.
+unfold tarray.
+erewrite split2_data_at_Tarray.
+3: rewrite sublist_same; [eassumption | auto | auto ].
+3: rewrite sublist_app1.
+3: rewrite sublist_same; [eassumption | auto | auto ].
+5: rewrite sublist_app2.
+5: rewrite sublist_same; [eassumption | auto | auto ].
+auto.
+all: rewrite Zlength_app in H; rep_omega.
+Qed.
+
+Lemma split_data_at_app_tschar:
+ forall sh n (al bl: list val) p ,
+   n = Zlength (al++bl) ->
+   data_at sh (tarray tschar n) (al++bl) p = 
+         data_at sh (tarray tschar (Zlength al)) al p
+        * data_at sh (tarray tschar (n - Zlength al)) bl
+                 (field_address0 (tarray tschar n) [ArraySubsc (Zlength al)] p).
+Proof.
+intros.
+apply (split_data_at_app sh tschar n al bl (al++bl)); auto.
+Qed.
+
+Lemma body_strcat: semax_body Vprog Gprog f_strcat strcat_spec.
+Proof.
+start_function.
+unfold cstringn, cstring in *.
+Intros.
+set (ld := string_to_Z sd) in *.
+set (ls := string_to_Z ss) in *.
+forward.
+forward_loop (EX i : Z,
+    PROP (0 <= i < Zlength ld + 1)
+    LOCAL (temp _i (Vint (Int.repr i)); temp _dest dest; temp _src src)
+    SEP (data_at Tsh (tarray tschar n)
+          (map Vint (map Int.repr (ld ++ [0])) ++
+           list_repeat (Z.to_nat (n - (Zlength ld + 1))) Vundef) dest;
+   data_at Tsh (tarray tschar (Zlength ls + 1))
+     (map Vint (map Int.repr (ls ++ [0]))) src))
+  break: (PROP ( )
+   LOCAL (temp _i (Vint (Int.repr (Zlength ld))); temp _dest dest; 
+   temp _src src)
+   SEP (data_at Tsh (tarray tschar n)
+          (map Vint (map Int.repr (ld ++ [0])) ++
+           list_repeat (Z.to_nat (n - (Zlength ld + 1))) Vundef) dest;
+   data_at Tsh (tarray tschar (Zlength ls + 1))
+     (map Vint (map Int.repr (ls ++ [0]))) src)).
+-
+  Exists 0; entailer!.
+-
+  Intros i.
+  forward.
+  pose proof (repable_string_i sd i) as Hi; fold ld in Hi.
+  forward.
+  { entailer!. }
+  { entailer!.
+    autorewrite with sublist. 
+    rewrite Znth_map with (d':= Int.zero) by list_solve.
+    rewrite Znth_map with (d':= 0) by list_solve.
+    simpl. normalize. }
+  autorewrite with sublist; simpl.
+  rewrite Znth_map with (d':= Int.zero) by list_solve.
+  rewrite Znth_map with (d':= 0) by list_solve.
+  forward.
+  forward_if_prop (Znth i (ld ++ [0]) 0 <> 0).
+  + forward.
+    entailer!. f_equal. f_equal. cstring.
+  +
+    forward.
+    entailer!. 
+  +
+    forward. Exists (i+1). entailer!. cstring.
+-
+  abbreviate_semax.
+  forward.
+  forward_loop (EX j : Z,
+    PROP (0 <= j < Zlength ls + 1)
+    LOCAL (temp _j (Vint (Int.repr j)); temp _i (Vint (Int.repr (Zlength ld)));
+           temp _dest dest; temp _src src)
+    SEP (data_at Tsh (tarray tschar n)
+          (map Vint (map Int.repr (ld ++ sublist 0 j ls)) ++
+           list_repeat (Z.to_nat (n - (Zlength ld + j))) Vundef) dest;
+         data_at Tsh (tarray tschar (Zlength ls + 1))
+           (map Vint (map Int.repr (ls ++ [0]))) src)).
+  { Exists 0; entailer!.  autorewrite with sublist.
+    rewrite !map_app. rewrite <- app_assoc.
+    rewrite split_data_at_app_tschar by list_solve.
+    rewrite (split_data_at_app_tschar _ n) by list_solve.
+    autorewrite with sublist.
+    cancel.    
+   }
+  { Intros j.
+  forward.
+  assert (Zlength (ls ++ [0]) = Zlength ls + 1) by (autorewrite with sublist; auto).
+  pose proof (repable_string_i ss j) as Hj; fold ls in Hj.
+  forward.
+  forward.
+  forward.
+  entailer!.
+  clear H3.
+  rewrite upd_Znth_app2 by list_solve.
+  autorewrite with sublist.
+  forward_if_prop (Znth j (ls ++ [0]) 0 <> 0).
+  + forward.
+      clear H8 H9 H6 PNdest PNsrc.
+      rewrite string_to_Z_app; autorewrite with sublist. fold ld. fold ls.
+      rewrite prop_true_andp 
+        by (intro Hx; apply in_app in Hx; destruct Hx; contradiction).
+      cancel.
+    assert (j = Zlength ls) by cstring; subst.
+    autorewrite with sublist.
+    apply derives_refl'.
+    unfold data_at; f_equal. 
+    replace (n - (Zlength ld + Zlength ls))
+     with (1 + (n - (Zlength ld + Zlength ls+1))) by rep_omega.
+    rewrite <- list_repeat_app' by rep_omega.
+    rewrite upd_Znth_app1 by list_solve.
+    rewrite app_assoc.
+    simpl.
+    rewrite !map_app.
+    reflexivity.
+ +
+  forward. entailer!.
+ +
+  forward.
+  Exists (j+1).
+  destruct (zlt j (Zlength ls)); [ | cstring].
+  entailer!.
+  change (field_at Tsh (tarray tschar n) []) with (data_at Tsh (tarray tschar n)).
+  rewrite (sublist_split 0 j (j+1)) by rep_omega.
+  rewrite (app_assoc ld). rewrite !map_app.
+  rewrite <- (app_assoc (_ ++ _)).
+  rewrite (split_data_at_app_tschar _ n) by list_solve.
+  rewrite (split_data_at_app_tschar _ n) by list_solve.
+  replace (n - (Zlength ld + j))
+    with (1 + (n - (Zlength ld + (j + 1)))) by rep_omega.
+  rewrite <- list_repeat_app' by rep_omega.
+  cancel.
+  rewrite upd_Znth_app1 by (autorewrite with sublist; rep_omega).
+  rewrite app_Znth1 by list_solve.
+  rewrite sublist_len_1 with (d:=0) by rep_omega.
+  cancel.
+}
+Qed.
+
+Lemma body_strcmp: semax_body Vprog Gprog f_strcmp strcmp_spec.
+Proof.
+start_function.
+unfold cstring in *.
+set (ls1 := string_to_Z s1).
+set (ls2 := string_to_Z s2).
+forward.
+Intros.
+forward_loop (EX i : Z,
+  PROP (0 <= i < Zlength ls1 + 1; 0 <= i < Zlength ls2 + 1;
+        sublist 0 i ls1 = sublist 0 i ls2)
+  LOCAL (temp _str1 str1; temp _str2 str2; temp _i (Vint (Int.repr i)))
+  SEP (data_at Tsh (tarray tschar (Zlength ls1 + 1))
+          (map Vint (map Int.repr (ls1 ++ [0]))) str1;
+       data_at Tsh (tarray tschar (Zlength ls2 + 1))
+          (map Vint (map Int.repr (ls2 ++ [0]))) str2)).
+- Exists 0; entailer!.
+- Intros i.
+  pose proof (repable_string_i s1 i) as Hi1; fold ls1 in Hi1.
+  pose proof (repable_string_i s2 i) as Hi2; fold ls2 in Hi2.
+  forward.
+  assert (Zlength (ls1 ++ [0]) = Zlength ls1 + 1) by (autorewrite with sublist; auto).
+  forward.
+  assert (Zlength (ls2 ++ [0]) = Zlength ls2 + 1) by (autorewrite with sublist; auto).
+  forward.
+  assert (Znth i (ls1 ++ [0]) 0 = 0 <-> i = Zlength ls1) as Hs1.
+  { split; [|intro; subst; rewrite app_Znth2, Zminus_diag by omega; auto].
+    destruct (zlt i (Zlength ls1)); [|omega].
+    intro X; lapply (Znth_In i ls1 0); [|omega]. cstring. }
+  assert (Znth i (ls2 ++ [0]) 0 = 0 <-> i = Zlength ls2) as Hs2.
+  { split; [|intro; subst; rewrite app_Znth2, Zminus_diag by omega; auto].
+    destruct (zlt i (Zlength ls2)); [|omega].
+    intro X; lapply (Znth_In i ls2 0); [|omega]. cstring. }
+  forward.
+  forward.
+  match goal with |-semax _ (PROP () (LOCALx ?Q ?R)) _ _ =>
+    forward_if (PROP ()
+      (LOCALx (temp _t'1 (Val.of_bool (Z.eqb i (Zlength ls1) && Z.eqb i (Zlength ls2))) :: Q) R)) end.
+  { forward.
+    simpl force_val.
+    rewrite Hs1 in *.
+    destruct (zeq (Znth i (ls2 ++ [0]) 0) 0).
+    + rewrite e; simpl force_val.
+         assert (i = Zlength ls2) by cstring.
+        rewrite  (proj2 Hs1 H6).
+     rewrite (proj2 (Z.eqb_eq i (Zlength ls1)) H6).
+     rewrite (proj2 (Z.eqb_eq i (Zlength ls2)) H7).
+     entailer!.
+  +
+    rewrite Int.eq_false.
+     rewrite (proj2 (Z.eqb_eq i (Zlength ls1)) H6).
+     rewrite Hs2 in n.
+     rewrite (proj2 (Z.eqb_neq i (Zlength ls2))) by auto.
+    entailer!.
+     contradict n.
+     apply repr_inj_signed; auto; red; rep_omega.
+ }
+  { forward.
+    entailer!.
+    destruct (i =? Zlength ls1) eqn: Heq; auto.
+    rewrite Z.eqb_eq in Heq; tauto. }
+  forward_if_prop ((i <> Zlength ls1 \/ i <> Zlength ls2) 
+                          /\  Znth i (ls1 ++ [0]) 0 = Znth i (ls2 ++ [0]) 0).
+ +
+  rewrite andb_true_iff in H6; destruct H6.
+  rewrite Z.eqb_eq in H6,H7.
+  forward.
+  Exists (Int.repr 0).
+  entailer!. simpl.
+  autorewrite with sublist in H3. subst ls1 ls2.
+  apply string_to_Z_inj; auto.
+ +
+  rewrite H6.
+  rewrite andb_false_iff in H6. rewrite !Z.eqb_neq in H6.
+  forward_if.
+  *
+    forward. Exists (Int.repr (-1)). entailer!.
+    simpl. intro; subst.
+    assert (ls1=ls2) by reflexivity.
+    rewrite <- H16 in *.
+    clear - H7; omega.
+ *
+   forward_if.
+   forward.
+   Exists (Int.repr 1). entailer!. simpl. intro. subst s2.
+   assert (ls1=ls2) by reflexivity.
+   rewrite <- H17 in *.
+   clear - H8; omega.
+   forward.
+   entailer!.
+   clear - H6.
+   destruct H6; rewrite <- Z.eqb_neq in H; rewrite H.
+   reflexivity. rewrite andb_comm. reflexivity.
++
+   forward.
+   Exists (i+1).
+   entailer!.
+  rewrite (sublist_split 0 i (i+1)) by omega.
+  rewrite (sublist_split 0 i (i+1)) by omega.
+  f_equal; auto.
+  rewrite !sublist_len_1 with (d:=0) by omega.
+  f_equal.
+  assert (i < Zlength ls2) by list_solve.
+  rewrite !app_Znth1 in H7 by list_solve. auto.
+Qed.
+
+Lemma body_strcpy: semax_body Vprog Gprog f_strcpy strcpy_spec.
+Proof.
+start_function.
+unfold cstring,cstringn in *.
+set (ls := string_to_Z s) in *.
+forward.
+Intros.
+forward_loop (EX i : Z,
+  PROP (0 <= i < Zlength ls + 1)
+  LOCAL (temp _i (Vint (Int.repr i)); temp _dest dest; temp _src src)
+  SEP (data_at Tsh (tarray tschar n)
+        (map Vint (map Int.repr (sublist 0 i ls)) ++ list_repeat (Z.to_nat (n - i)) Vundef) dest;
+       data_at Tsh (tarray tschar (Zlength ls + 1)) (map Vint (map Int.repr (ls ++ [0]))) src)).
+*
+ Exists 0. rewrite Z.sub_0_r; entailer!.
+*
+ Intros i.
+ pose proof (repable_string_i s i) as Hi; fold ls in Hi.
+ forward.
+ assert (Zlength (ls ++ [0]) = Zlength ls + 1) by (autorewrite with sublist; auto).
+ forward.
+ forward.
+ forward.
+ forward_if_prop (Znth i (ls ++ [0]) 0 <> 0).
++
+   forward.
+   entailer!.
+   assert (i = Zlength ls) by cstring. subst i.
+   change (field_at Tsh (tarray tschar n) []) with (data_at Tsh (tarray tschar n)).
+   rewrite upd_Znth_app2 by list_solve.
+   autorewrite with sublist.
+   rewrite !map_app.
+   rewrite <- app_assoc.
+   rewrite (split_data_at_app_tschar _ n) by list_solve.
+   rewrite (split_data_at_app_tschar _ n) by list_solve.
+   autorewrite with sublist.
+   replace (n - Zlength ls) with (1 + (n - (Zlength ls + 1))) at 2 by list_solve.
+   rewrite <- list_repeat_app' by omega.
+   rewrite upd_Znth_app1 by list_solve.
+   rewrite !split_data_at_app_tschar by list_solve.
+   cancel.
++
+   assert (i < Zlength ls) by cstring.
+   forward.
+   entailer!.
++
+   forward.
+   Exists (i+1). entailer!. cstring.
+   rewrite upd_Znth_app2 by list_solve.
+   assert (i < Zlength ls) by cstring.
+   rewrite (sublist_split 0 i (i+1)) by list_solve. 
+   rewrite !map_app. rewrite <- app_assoc.
+   autorewrite with sublist.
+   change (field_at Tsh (tarray tschar n) []) with (data_at Tsh (tarray tschar n)).
+   rewrite !(split_data_at_app_tschar _ n) by list_solve.
+   autorewrite with sublist.
+   replace (n - i) with (1 + (n-(i+ 1))) at 2 by list_solve.
+   rewrite <- list_repeat_app' by omega.
+   rewrite upd_Znth_app1 by list_solve.
+   cancel.
+   rewrite !split_data_at_app_tschar by list_solve.
+   autorewrite with sublist.
+   rewrite sublist_len_1 with (d:=0) by omega.
+   simpl. cancel.
+Qed.
+
+End Alternate.
+
 
